{
 "cells": [
  {
   "cell_type": "markdown",
   "metadata": {},
   "source": [
    "# Exercise 3.1.1a (C3-P1)\n",
    "\n",
    "## Use Lagrange interpolation to find a polynomial that passes through the points $(0, 1), (2, 3), (3, 0)$.\n",
    "\n",
    "The Lagrange interpolation polynomial for three points $(x_1, y_1), (x_2, y_2),$ and $(x_3, y_3)$ is given by the formula:\n",
    "\n",
    "$$P(x) = y_1 \\frac{(x - x_2)(x - x_3)}{(x_1 - x_2)(x_1 - x_3)} + y_2 \\frac{(x - x_1)(x - x_3)}{(x_2 - x_1)(x_2 - x_3)} + y_3 \\frac{(x - x_1)(x - x_2)}{(x_3 - x_1)(x_3 - x_2)}$$\n",
    "\n",
    "The points are:\n",
    "\n",
    "- $(x_1, y_1) = (0, 1)$\n",
    "- $(x_2, y_2) = (2, 3)$\n",
    "- $(x_3, y_3) = (3, 0)$\n",
    "\n",
    "### Step-by-step calculation:\n",
    "\n",
    "1. **First term** (corresponding to $(x_1, y_1) = (0, 1)$):\n",
    "\n",
    "$$\n",
    "1 \\cdot \\frac{(x - 2)(x - 3)}{(0 - 2)(0 - 3)} = 1 \\cdot \\frac{(x - 2)(x - 3)}{(-2)(-3)} = \\frac{(x - 2)(x - 3)}{6}\n",
    "$$\n",
    "\n",
    "2. **Second term** (corresponding to $(x_2, y_2) = (2, 3)$)\n",
    "\n",
    "$$\n",
    "3 \\cdot \\frac{(x - 0)(x - 3)}{(2 - 0)(2 - 3)} = 3 \\cdot \\frac{(x)(x - 3)}{(2)(-1)} = -\\frac{3x(x - 3)}{2}\n",
    "$$\n",
    "\n",
    "3. **Third term** (corresponding to $(x_3, y_3) = (3, 0)$):\n",
    "\n",
    "$$\n",
    "0 \\cdot \\frac{(x - 0)(x - 2)}{(3 - 0)(3 - 2)} = 0\n",
    "$$\n",
    "\n",
    "### Combine the terms:\n",
    "\n",
    "$$\n",
    "P(x) = \\frac{(x - 2)(x - 3)}{6} - \\frac{3x(x - 3)}{2}\n",
    "$$\n",
    "\n",
    "### Simplify:\n",
    "\n",
    "First term:\n",
    "\n",
    "$$\n",
    "\\frac{(x - 2)(x - 3)}{6} = \\frac{x^2 - 5x + 6}{6}\n",
    "$$\n",
    "\n",
    "Second term:\n",
    "\n",
    "$$\n",
    "-\\frac{3x(x - 3)}{2} = -\\frac{3(x^2 - 3x)}{2} = -\\frac{3x^2}{2} + \\frac{9x}{2}\n",
    "$$\n",
    "\n",
    "Now, combine these two terms:\n",
    "\n",
    "$$\n",
    "P(x) = \\frac{x^2 - 5x + 6}{6} - \\left(\\frac{3x^2}{2} - \\frac{9x}{2}\\right)\n",
    "$$\n",
    "\n",
    "To combine, first rewrite everything with a denominator of 6:\n",
    "\n",
    "$$\n",
    "P(x) = \\frac{x^2 - 5x + 6}{6} - \\frac{9x^2 - 27x}{6}\n",
    "$$\n",
    "\n",
    "Now simplify:\n",
    "\n",
    "$$\n",
    "P(x) = \\frac{x^2 - 5x + 6 - 9x^2 + 27x}{6}\n",
    "$$\n",
    "\n",
    "$$\n",
    "P(x) = \\frac{-8x^2 + 22x + 6}{6}\n",
    "$$\n",
    "\n",
    "This is the final polynomial:\n",
    "\n",
    "$$\n",
    "P(x) = \\frac{-4x^2 + 11x + 3}{3}\n",
    "$$\n",
    "\n",
    "This is the interpolating polynomial that passes through the points $(0, 1)$, $(2, 3)$, and $(3, 0)$.\n"
   ]
  }
 ],
 "metadata": {
  "language_info": {
   "name": "python"
  }
 },
 "nbformat": 4,
 "nbformat_minor": 2
}
